stuck

research/src/Scratch.v
@@ -1,1 +1,60 @@
-Require Import FL.CpdtTactics.
+Require Import Init.Nat Arith List FL.CpdtTactics.
+Require Import Logic.Decidable.
+Set Implicit Arguments.
+Set Asymmetric Patterns.
+
+Inductive Term : Set := 
+    | NumTerm : nat -> Term
+    | Plus : Term -> Term -> Term
+    .
+
+Fixpoint termDenote (t : Term) : nat := 
+match t with
+| NumTerm n => n
+| Plus n n' => (termDenote n) + (termDenote n')
+end.
+
+Eval simpl in termDenote (Plus (Plus (NumTerm 0) (NumTerm 5)) (NumTerm 7)).
+
+Inductive RelOp : Set := 
+    | Eq
+    | Lt
+    | Lte
+    . 
+
+Definition relOpDenote (r : RelOp) : nat -> nat -> Prop :=
+match r with
+| Eq => eq
+| Lt => lt
+| Lte => le
+end.
+
+Inductive Formula : Set := 
+    | And : Formula -> Formula -> Formula
+    | Or : Formula -> Formula -> Formula
+    | Not : Formula -> Formula
+    | ForAll : (nat -> Formula) -> Formula
+    | Exists : (nat -> Formula) -> Formula
+    | Rel : Term -> RelOp -> Term -> Formula
+    .
+
+Fixpoint formDenote (f : Formula) : Prop := 
+match f with
+    | And f1 f2 => (formDenote f1) /\ (formDenote f2)
+    | Or f1 f2 => (formDenote f1) \/ (formDenote f2)
+    | Not f1 => ~ (formDenote f1)
+    | Rel t1 rel t2 => (relOpDenote rel) (termDenote t1) (termDenote t2)
+    | ForAll f' => forall n : nat, formDenote (f' n)
+    | Exists f' => exists n : nat, formDenote(f' n)
+end.
+
+Theorem formulas_are_decidable : forall (f : Formula) (p : Prop),
+  formDenote f = p ->
+  decidable p.
+Proof.
+intros f.
+induction f.
+- crush.
+- crush.
+- crush.
+- simpl. intros. apply p in H.
